clean up

theories/ccompiler/equiv.v
@@ -1,5 +1,5 @@
 From Wasm Require Import datatypes.
-From Wasm Require Import ccompiler.compile.
+From Wasm Require Import ccompiler.compile ccompiler.num_conv.
 Require Import compcert.lib.Integers.
 Require Import compcert.cfrontend.Clight.
 Require Import compcert.common.AST.
@@ -8,8 +8,8 @@ Require Import compcert.common.Values.
 
 Definition val_equiv (v : value) : val :=
   match v with
-  | VAL_int32 x => Vint (Integers.Int.mkint (Wasm_int.Int32.intval x) (Wasm_int.Int32.intrange x))
-  | VAL_int64 x => Vlong (Integers.Int64.mkint (Wasm_int.Int64.intval x) (Wasm_int.Int64.intrange x))
+  | VAL_int32 x => Vint (int_of x)
+  | VAL_int64 x => Vlong (long_of x)
   | VAL_float32 x => Vsingle x
   | VAL_float64 x => Vfloat x
   end.
@@ -17,7 +17,7 @@ Definition val_equiv (v : value) : val :=
 Lemma lit_equiv :
   forall (ge : genv) (e : env) (te : temp_env) (m : mem),
   forall (c : value),
-  eval_expr ge e te m (fst (compile_const' c)) (val_equiv c).
+  eval_expr ge e te m (compile_value c) (val_equiv c).
 Proof.
-  intros; unfold compile_const'; destruct c; eauto using eval_expr.
+  intros. unfold compile_value. destruct c; eauto using eval_expr.
 Qed.
