theories/ccompiler/num_conv.v
@@ -1,0 +1,10 @@
+From Wasm Require Import numerics.
+From compcert Require Import Integers.
+
+Definition int_of (x : Wasm_int.Int32.int) : int :=
+  Integers.Int.mkint
+    (Wasm_int.Int32.intval x) (Wasm_int.Int32.intrange x).
+
+Definition long_of (x : Wasm_int.Int64.int) : int64 :=
+  Integers.Int64.mkint
+    (Wasm_int.Int64.intval x) (Wasm_int.Int64.intrange x).
